aneris/examples/transactional_consistency/read_committed/trace/implication_trace.v
@@ -1,4 +1,4 @@
-From iris.algebra Require Import gset auth gmap excl excl_auth csum.
+From iris.algebra Require Import gset auth frac_auth gmap excl excl_auth csum.
 From iris.base_logic.lib Require Import mono_nat ghost_map.
 From iris.algebra.lib Require Import mono_list.
 From aneris.algebra Require Import monotone.
@@ -9,45 +9,927 @@ From aneris.aneris_lang.lib.serialization Require Import serialization_proof.
 From aneris.aneris_lang.program_logic Require Import lightweight_atomic.
 From aneris.examples.transactional_consistency Require Import code_api wrapped_library.
 From aneris.examples.transactional_consistency.read_committed.specs Require Import specs resources.
-From aneris.examples.transactional_consistency Require Import user_params aux_defs state_based_model.
+From aneris.examples.transactional_consistency 
+  Require Import resource_algebras user_params aux_defs state_based_model implication_trace_util.
 
 Section trace_proof.
-  Context `{!User_params}.
+  Context `{!anerisG Mdl Σ, !KVSG Σ, !User_params}.
+
+  Definition OwnTransSub (γ : gname) (trans : transaction) : iProp Σ :=
+    ∃ (T : list transaction), own γ (◯ (gmap_of_trace 0 T)) ∗ ⌜trans ∈ T⌝.
+
+  Definition OwnTrans (γ : gname) (T : list transaction) : iProp Σ :=
+    own γ (● gmap_of_trace 0 T) ∗ own γ (◯ (gmap_of_trace 0 T)).
+
+  Lemma own_trans (γ : gname) (T : list transaction) (trans : transaction) :
+    OwnTrans γ T ==∗ OwnTrans γ (T ++ [trans]) ∗ OwnTransSub γ trans.
+  Proof.
+    rewrite /OwnTrans /OwnTransSub.
+    iIntros "(H1 & #H2)".
+    rewrite gmap_of_trace_snoc Nat.add_0_l.
+    iMod (own_update_2 with "H1 H2") as "[H1 H3]".
+    apply auth_update.
+    eapply (alloc_local_update (gmap_of_trace 0 T) (gmap_of_trace 0 T) 
+      (length T : nat) (to_agree (trans : transaction))); try done.
+    { 
+      eapply not_elem_of_dom.
+      rewrite gmap_of_trace_dom.
+      intro Hfalse. 
+      lia. 
+    }
+    iDestruct "H3" as "#H4".
+    iModIntro.
+    iFrame "∗#".
+    iExists (T ++ [trans]).
+    rewrite gmap_of_trace_snoc Nat.add_0_l.
+    iFrame "#".
+    iPureIntro.
+    set_solver.
+  Qed.
+
+  Lemma own_trans_in (γ : gname) (T : list transaction) (trans : transaction):
+    OwnTrans γ T ∗ OwnTransSub γ trans -∗
+    OwnTrans γ T ∗ OwnTransSub γ trans ∗ ⌜trans ∈ T⌝.
+  Proof.
+    rewrite /OwnTrans /OwnTransSub.
+    iIntros "((H1 & #H2) & (%T' & #H3 & %Hin))".
+    iDestruct (own_op with "[$H1 $H3]") as "H".
+    iDestruct (own_valid with "H") as %[Hsub Hvalid]%auth_both_valid_discrete.
+    iDestruct "H" as "(H1 & _)".
+    iFrame "#∗".
+    iSplit; first set_solver.
+    iPureIntro.
+    assert (T' `prefix_of` T) as Hprefix.
+    - eapply gmap_of_trace_hist_valid_prefix; eauto.
+    - by eapply elem_of_prefix.
+  Qed.
+
+  Definition GlobalInvExtRC (γ : gname) (T : list transaction) : iProp Σ := 
+    OwnTrans γ (comTrans T) ∗ 
+      ⌜∀ trans s k v, trans ∈ T → (Rd s k (Some v)) ∈ trans → 
+        ¬(∃ s, (Wr s k v) ∈ trans) → ∃ trans', trans' ∈ (comTrans T) ∧ latest_write_trans k v trans'⌝.
 
   (** Wrapped resources  *)
-  Global Program Instance wrapped_resources `{!anerisG Mdl Σ} `(res : !RC_resources Mdl Σ) : RC_resources Mdl Σ :=
+  Global Program Instance wrapped_resources (γtrans γmstate γmlin γmpost γmname γl : gname) (clients : gset socket_address) 
+  `(res : !RC_resources Mdl Σ) : RC_resources Mdl Σ :=
     {|
-      GlobalInv := True%I;
-      OwnMemKey k V := True%I;
-      OwnLocalKey k c vo := True%I;
-      ConnectionState c s sa := True%I;
-      IsConnected c sa := True%I;
+      GlobalInv := (GlobalInv ∗ trace_inv trace_inv_name valid_trace_rc ∗ 
+                    inv KVS_InvName (∃ T, GlobalInvExtRC γtrans T ∗ GlobalInvExt T extract γmstate γmlin γmpost γmname γl clients))%I;
+      OwnMemKey k V :=  (OwnMemKey k V ∗ 
+                        (* This part captures the RC test in the model *)
+                        (∀ v, ⌜v ∈ V⌝ → ∃ trans, OwnTransSub γtrans trans ∗ ⌜latest_write_trans k v trans⌝ ∗ ⌜com_true trans⌝) ∗
+                        (* This part captures correct extraction *)
+                        (∀ v, ⌜v ∈ V⌝ → ∃ lh tag c, OwnLinHist γl lh ∗ 
+                        ⌜(#(LitString tag), (c, (#"WrLin", (#(LitString k), v))))%V ∈ lh⌝))%I;
+      OwnLocalKey k c ov := (OwnLocalKey k c ov ∗ ∃ (sa : socket_address) γ, ghost_map_elem γmname sa DfracDiscarded (γ, c) ∗ 
+                             ⌜extract c = Some #sa⌝ ∗ (⌜k ∈ KVS_keys⌝ → ghost_map_elem γ k (DfracOwn 1%Qp) ov) ∗ ⌜sa ∈ clients⌝)%I;
+      ConnectionState c sa s := (ConnectionState c sa s ∗ ghost_map_elem γmstate sa (DfracOwn 1%Qp) (s, Some c))%I;
+      IsConnected c sa := (IsConnected c sa ∗ ⌜sa ∈ clients⌝ ∗ ⌜extract c = Some #sa⌝ ∗ 
+                           ∃ γ, ghost_map_elem γmname sa DfracDiscarded (γ, c))%I;
       KVS_rc := KVS_rc;
-      KVS_Init := True%I;
-      KVS_ClientCanConnect sa := True%I;
-      Seen k V := True%I;
+      KVS_Init := KVS_Init%I;
+      KVS_ClientCanConnect sa := (KVS_ClientCanConnect sa ∗ ghost_map_elem γmstate sa (DfracOwn 1%Qp) (CanStart, None) ∗ ⌜sa ∈ clients⌝)%I;
+      Seen k V := Seen k V%I;
       extract c := res.(read_committed.specs.resources.extract) c;
     |}.
   Next Obligation.
-  Admitted.
+    iIntros (???????????) "(Hkey & [%sa [%γ (Hghost_elem_per & %Hextract & Hghost_elem  & %Hin_sa)]])".
+    iDestruct (res.(read_committed.specs.resources.OwnLocalKey_serializable) 
+      with "Hkey") as "(Hkey & Hser)".
+    iFrame.
+    iExists sa, γ.
+    by iFrame.
+  Qed.
   Next Obligation.
-  Admitted.
+    iIntros (?????????????) "#(HGinv & Hinv) (#Hseen & Hkey & Hin)".
+    iMod (res.(read_committed.specs.resources.Seen_valid) 
+      with "[$HGinv][$Hseen $Hkey]") as "(Hkey & Hsub)"; first done.
+    iModIntro.
+    iFrame "∗#".
+  Qed.
   Next Obligation.
-  Admitted.
+    iIntros (????????????) "#(HGinv & Hinv) (Hkey & Hin)".
+    iMod (res.(read_committed.specs.resources.Seen_creation) 
+      with "[$HGinv][$Hkey]") as "(Hkey & #Hseen)"; first done.
+    iModIntro.
+    iFrame "∗#".
+  Qed.
   Next Obligation.
-  Admitted.
+    simpl.
+    iIntros (?????? clients res sa c) "(Hconn & _)".
+    iApply (res.(read_committed.specs.resources.Extraction_of_address) 
+      with "[$Hconn]").
+  Qed.
   Next Obligation.
+    simpl.
+    iIntros (?????? clients res sa sa' c c' Heq1 Heq2 Hneq).
+    by eapply res.(read_committed.specs.resources.Extraction_preservation).
+  Qed.
+
+  (** Per operation implications *)
+
+  Lemma init_client_implication γtrans γmstate γmlin γmpost γmname γl clients (res : RC_resources Mdl Σ) 
+  (lib : KVS_transaction_api) : 
+    ⌜KVS_InvName = nroot .@ "kvs_inv"⌝ -∗
+    trace_inv trace_inv_name valid_trace_rc -∗
+    inv KVS_InvName (∃ T, GlobalInvExtRC γtrans T ∗ GlobalInvExt T extract γmstate γmlin γmpost γmname γl clients) -∗
+    @init_client_proxy_spec _ _ _ _ lib res -∗
+    @init_client_proxy_spec _ _ _ _ (KVS_wrapped_api lib) (wrapped_resources γtrans γmstate γmlin γmpost γmname γl clients res).
+  Proof.
+    iIntros "%Hkvs_inv_name #Htr_inv #HinvExt #Hinit_cli".
+    rewrite /init_client_proxy_spec.
+    iIntros (sa Φ) "!# (Hunall & Hsock & Hmes & (Hcan & (Hsa_pointer & %Hsa_in)) & Hfree) HΦ".
+    rewrite /TC_init_client_proxy /KVS_wrapped_api /wrap_init_client_proxy.
+    wp_pures.
+    wp_bind (ast.Fresh _).
+    iInv "HinvExt" as ">[%T (Htrans_res & [%t [%lt (Htr_is & HOwnLin & %HlinOf & %Hno_empty & %Hex 
+      & %Hvalid_trans & %Hvalid_seq & Hstate_res & Hlin_res & Hpost_res)]])]" "Hclose".
+    wp_apply (aneris_wp_fresh with "[$Htr_inv $Htr_is]").
+    {
+      rewrite Hkvs_inv_name.
+      solve_ndisj.
+    }
+    {
+      intros tag Hnin.
+      (* eapply valid_trace_rc_pre; try done.
+      rewrite /is_pre_event /is_in_pre_event; set_solver. *)
+      admit.
+    }
+    iIntros (tag1) "(Htr_is & %Htag1_nin)".
+    rewrite /init_pre_emit_event.
+    iDestruct (alloc_trace_hist with "[$Htr_is]") as "(Htr_is & #Htr_hist)".
+    iMod (lin_tag_create lt t γmlin (#tag1, init_pre_emit_event)%V with "[$Hlin_res]") 
+      as "(Hlin_res & Hlin_tag_res)".
+    {
+      iPureIntro.
+      simpl.
+      do 2 (split; first done).
+      intros Hfalse.
+      destruct Hfalse as [Hfalse | [[Hfalse | Hfalse] | [Hfalse | [Hfalse | Hfalse]]]]; 
+        rewrite /is_st_post_event /is_wr_post_event /is_cm_post_event /is_in_post_event in Hfalse; 
+        set_solver.
+    }
+    iMod (post_tag_create t γmpost (#tag1, init_pre_emit_event)%V with "[$Hpost_res]") 
+      as "(Hpost_res & Hpost_tag_res)".
+    {
+      iPureIntro.
+      simpl.
+      do 2 (split; first done).
+      intros Hfalse.
+      destruct Hfalse as [Hfalse | [[Hfalse | Hfalse] | [Hfalse | [Hfalse | Hfalse]]]]; 
+        rewrite /is_st_post_event /is_wr_post_event /is_cm_post_event /is_in_post_event in Hfalse; 
+        set_solver.
+    }
+    iMod ("Hclose" with "[Htrans_res Htr_is HOwnLin Hlin_res Hpost_res Hstate_res]").
+    {
+      iNext.
+      iExists T.
+      iFrame.
+      iExists (t ++ [(#tag1, init_pre_emit_event)%V]), lt.
+      iFrame.
+      iSplitR; last set_solver.
+      iPureIntro.
+      apply (lin_trace_valid tag1); try done.
+      rewrite /is_pre_event /is_in_pre_event.
+      set_solver.
+    }
+    iModIntro.
+    wp_pures.
+    wp_apply ("Hinit_cli" $! sa with "[$Hunall $Hsock $Hmes $Hcan $Hfree]").
+    iIntros (c) "(Hconn_state & #His_conn)".
+    wp_pures.
+    wp_bind (ast.Emit _).
+    rewrite /init_post_emit_event.
+    wp_pures.
+    iInv "HinvExt" as ">[%T' (Htrans_res' & [%t' [%lt' (Htr_is' & HOwnLin' & %HlinOf' & %Hno_empty' & %Hex' 
+      & %Hvalid_trans' & %Hvalid_seq' & Hstate_res' & Hlin_res' & Hpost_res')]])]" "Hclose'".
+    iMod (own_lin_add _ _ (#tag1, (c, #"InLin"))%V with "[$HOwnLin']") as "HOwnLin'".
+    iPoseProof (trace_hist_trace_is_prefix with "[$Htr_is'][$Htr_hist]") as "%Hprefix".
+    assert ((#tag1, #"InPre")%V ∈ t') as Hin'.
+    {
+      apply (elem_of_prefix (t ++ [(#tag1, #"InPre")%V])); last done.
+      set_solver.
+    }
+    iPoseProof (lin_tag_not_in lt' t' γmlin with "[$Hlin_res' $Hlin_tag_res]") as "%Hnot_lin_in".
+    iPoseProof (post_tag_not_in t' γmpost with "[$Hpost_res' $Hpost_tag_res]") as "%Hnot_post_in".
+    iDestruct (lin_tag_add lt' t' γmlin (#tag1, (c, #"InLin"))%V tag1 with "[$Hlin_res' $Hlin_tag_res]") 
+      as "Hlin_res'".
+    {
+      iPureIntro.
+      by simpl.
+    }
+    iDestruct "Hstate_res'" as "[%mstate (Hghost_map_mstate & [%mname (Hghost_map_mname & Hext_rest1')])]".
+    iDestruct (@ghost_map_lookup with "[$Hghost_map_mstate][$Hsa_pointer]") as "%Hlookup".
+    assert (clients = {[sa]} ∪ (clients ∖ {[sa]})) as Heq_sa_clients.
+    {
+      apply union_difference_L.
+      set_solver.
+    }
+    rewrite {4} Heq_sa_clients.
+    rewrite (big_sepS_union _ {[sa]} (clients ∖ {[sa]})); last set_solver.
+    iDestruct "Hext_rest1'" as "(Hext_rest1_sa & Hext_rest1)".
+    rewrite big_sepS_singleton.
+    iAssert ((⌜mname !! sa = None⌝ ∧ ⌜no_emit_with_address sa lt' extract⌝)%I) as "(%Hlookup_none & %Hno_emit)".
+    {
+      iDestruct ("Hext_rest1_sa") as "[(_ & %Hnot_lookup & %Hno_emit)|[%s [%c' [%γ [%m (%Hfalse & asd)]]]]]".
+      - iPureIntro. 
+        destruct (mname !! sa) as [γ|] eqn:Hfalse; last done.
+        exfalso.
+        apply Hnot_lookup.
+        by exists γ.
+      - set_solver.
+    }
+    iDestruct (res.(read_committed.specs.resources.Extraction_of_address) 
+          with "[$His_conn]") as "%Hextract".
+    assert (lin_trace_of (lt' ++ [(#tag1, (c, #"InLin"))%V])
+      (t' ++ [(#tag1, (c, #"InPost"))%V])) as Hlin_trace'.
+    {
+      apply (lin_trace_valid tag1); try done.
+      - right.
+        split.
+        + do 4 right. 
+          rewrite /is_in_post_event; eauto.
+        + exists (#tag1, (c, #"InLin"))%V.
+          set_solver.
+      - apply (lin_trace_lin lt' (#tag1, #"InPre")%V 
+          (#tag1, (c, #"InLin"))%V tag1 c t'); try done;
+          rewrite /is_lin_event /is_in_lin_event /is_pre_event /is_in_pre_event;
+          set_solver.
+    }
+    assert (valid_sequence (lt' ++ [(#tag1, (c, #"InLin"))%V])) as Hvalid_seq''.
+    {
+      apply valid_sequence_in_lin; try done.
+      eapply unique_init_events_add_init; try done.
+      rewrite /valid_sequence in Hvalid_seq'; set_solver.
+    }
+    wp_apply (aneris_wp_emit with "[$Htr_inv $Htr_is']").
+    {
+      rewrite Hkvs_inv_name.
+      solve_ndisj.
+    }
+    {
+      (* rewrite /valid_trace_rc /valid_trace.
+      exists (lt' ++ [(#tag1, (c, #"InLin"))%V]).
+      split_and!; try done.
+      destruct (exists_execution T') as [E' (Hbased' & Hvalid_exec')]; first set_solver.
+      eexists T', E'.
+      split_and!; try done.
+      apply extraction_of_add_init_lin; rewrite /is_in_lin_event;
+        set_solver. *)
+      admit.
+    }
+    iIntros "Htr_is".
+    iDestruct (lin_tag_add_post (lt' ++ [(#tag1, (c, #"InLin"))%V]) t' γmlin (#tag1, (c, #"InPost"))%V 
+      with "[$Hlin_res']") as "Hlin_res'".
+    iDestruct (post_tag_add t' γmpost (#tag1, (c, #"InPost"))%V tag1 with "[$Hpost_res' $Hpost_tag_res]")
+      as "Hpost_res'".
+    {
+      iPureIntro.
+      simpl.
+      split; first done.
+      do 4 right.
+      rewrite /is_in_post_event.
+      by eexists _, _.
+    }
+    iMod (ghost_map_alloc ((gset_to_gmap None KVS_keys : gmap Key (option val))))
+      as "[%γ (Hghost_map_m & Hghost_elems_m)]".
+    iMod (ghost_map_update (CanStart, Some c) with "[$Hghost_map_mstate] [$Hsa_pointer]") 
+      as "(Hghost_map_mstate & Hsa_pointer)".
+    iMod (ghost_map_insert_persist sa (γ, c) Hlookup_none with "[$Hghost_map_mname]") 
+      as "(Hghost_map_mname & #Hkey_pers_mname)".
+    iMod ("Hclose'" with "[Htrans_res' Htr_is HOwnLin' Hghost_map_mname Hext_rest1 Hext_rest1_sa 
+      Hghost_map_mstate Hghost_map_m Hghost_elems_m Hlin_res' Hpost_res']").
+    {
+      iNext.
+      iExists T'.
+      iFrame.
+      iExists (t' ++ [(#tag1, (c, #"InPost"))%V]), (lt' ++ [(#tag1, (c, #"InLin"))%V]).
+      iFrame.
+      do 2 (iSplit; first by iPureIntro).
+      iSplit; first iPureIntro.
+      {
+        apply extraction_of_add_init_lin; rewrite /is_in_lin_event;
+        set_solver.
+      }
+      do 2 (iSplit; first by iPureIntro).
+      iClear "HinvExt Hinit_cli Htr_inv".
+      iExists (<[sa:=(CanStart, Some c)]> mstate).
+      iFrame.
+      iExists (<[sa:=(γ, c)]> mname).
+      iFrame.
+      rewrite {2} Heq_sa_clients.
+      rewrite big_sepS_union; last set_solver.
+      iSplitL "Hghost_map_m Hghost_elems_m".
+      + iApply big_sepS_singleton.
+        iRight.
+        iExists CanStart, c, γ, (gset_to_gmap None KVS_keys).
+        rewrite lookup_insert.
+        iFrame "#∗".
+        do 2 (iSplit; first by iPureIntro).
+        iSplit.
+        {
+          iPureIntro.
+          exists (#tag1, (c, #"InLin"))%V.
+          simpl.
+          rewrite /is_in_lin_event.
+          split_and!; try done; eauto.
+          apply elem_of_app.
+          right.
+          set_solver.
+        }
+        iLeft.
+        iSplit; first by iPureIntro.
+        iSplit.
+        * iPureIntro.
+          rewrite /commit_closed.
+          intros e_st Hin Hconn Hstart.
+          exfalso.
+          apply Hno_emit.
+          assert (e_st ∈ lt') as Hin_st; last set_solver.
+          rewrite elem_of_app in Hin.
+          destruct Hin as [Hin|Hin]; first done.
+          rewrite /is_st_lin_event in Hstart.
+          set_solver.
+        * iSplit. 
+          -- iPureIntro. 
+             intros (trans & (op & Ht'_in & Hlast & Hconn_last & _)).
+             destruct Hex' as (_ & Hex' & _).
+             apply last_Some_elem_of in Hlast.
+             specialize (Hex' trans op Ht'_in Hlast).
+             apply Hno_emit.
+             exists (toLinEvent op), c.
+             split_and!; try done.
+             destruct op; destruct s; 
+              simpl in Hconn_last; subst; 
+              simpl; try done.
+              by destruct ov.
+          -- rewrite big_sepM_gset_to_gmap.
+             iApply (big_sepS_wand with "[$Hghost_elems_m]").
+             iApply big_sepS_intro.
+             iModIntro.
+             iIntros (k Hk_in) "Hkey".
+             iExists None.
+             iFrame.
+      + iApply (big_sepS_wand with "[$Hext_rest1]").
+        iApply big_sepS_intro.
+        iModIntro.
+        iIntros (sa' Hsa'_in) "Hext_res".
+        iApply (client_trace_state_resources_neq3 sa sa' c with "[][][][$]"); try done.
+        iPureIntro; set_solver.
+    }
+    iModIntro.
+    wp_pures.
+    iApply "HΦ".
+    rewrite /ConnectionState.
+    simpl.
+    iFrame "∗#".
+    do 2 (iSplit; first by iPureIntro).
+    iExists γ.
+    iFrame "#".
   Admitted.
 
-  Definition trace_inv_name := nroot.@"trinv".
+  Lemma read_implication γtrans γmstate γmlin γmpost γmname γl clients (res : RC_resources Mdl Σ) 
+  (lib : KVS_transaction_api) : 
+    ⌜KVS_InvName = nroot .@ "kvs_inv"⌝ -∗
+    trace_inv trace_inv_name valid_trace_rc -∗
+    inv KVS_InvName (∃ T, GlobalInvExtRC γtrans T ∗ GlobalInvExt T extract γmstate γmlin γmpost γmname γl clients) -∗
+    @read_spec _ _ _ _ lib res -∗
+    @read_spec _ _ _ _ (KVS_wrapped_api lib) (wrapped_resources γtrans γmstate γmlin γmpost γmname γl clients res).
+  Proof.
+  Admitted.
+
+  Lemma write_implication γtrans γmstate γmlin γmpost γmname γl clients (res : RC_resources Mdl Σ) 
+  (lib : KVS_transaction_api) : 
+    ⌜KVS_InvName = nroot .@ "kvs_inv"⌝ -∗
+    trace_inv trace_inv_name valid_trace_rc -∗
+    inv KVS_InvName (∃ T, GlobalInvExtRC γtrans T ∗ GlobalInvExt T extract γmstate γmlin γmpost γmname γl clients) -∗
+    @write_spec _ _ _ _ lib res -∗
+    @write_spec _ _ _ _ (KVS_wrapped_api lib) (wrapped_resources γtrans γmstate γmlin γmpost γmname γl clients res).
+  Proof.
+  Admitted.
+
+  Lemma start_implication γtrans γmstate γmlin γmpost γmname γl clients (res : RC_resources Mdl Σ) 
+  (lib : KVS_transaction_api) : 
+    ⌜KVS_InvName = nroot .@ "kvs_inv"⌝ -∗
+    trace_inv trace_inv_name valid_trace_rc -∗
+    inv KVS_InvName (∃ T, GlobalInvExtRC γtrans T ∗ GlobalInvExt T extract γmstate γmlin γmpost γmname γl clients) -∗
+    @start_spec _ _ _ _ lib res -∗
+    @start_spec _ _ _ _ (KVS_wrapped_api lib) (wrapped_resources γtrans γmstate γmlin γmpost γmname γl clients res).
+  Proof.
+    iIntros "%Hkvs_inv_name #Htr_inv #HinvExt #Hstart".
+    rewrite /start_spec.
+    iModIntro.
+    iIntros (c sa E) "%Hsub (#Hconn & %Hsa_in_clients & %Hsa_extract & #Hpers_pointer) !# %Φ Hshift".
+    rewrite /TC_start /KVS_wrapped_api /wrap_start.
+    wp_pures.
+    wp_bind (ast.Fresh _).
+    rewrite /start_pre_emit_event.
+    wp_pures.
+    iInv "HinvExt" as ">[%T (Htrans_res & [%t [%lt 
+      (Htr_is & HOwnLin & %HlinOf & %Hno_empty & %Hex & %Hvalid_trans & %Hvalid_seq 
+      & Hstate_res & Hlin_res & Hpost_res)]])]" "Hclose".
+    wp_apply (aneris_wp_fresh with "[$Htr_inv $Htr_is]").
+    {
+      rewrite Hkvs_inv_name.
+      solve_ndisj.
+    }
+    {
+      (* intros tag Hnin.
+      eapply valid_trace_ru_pre; try done.
+      rewrite /is_pre_event /is_st_pre_event; set_solver. *)
+      admit.
+    }
+    iIntros (tag1) "(Htr_is & %Htag1_nin)".
+    iDestruct (alloc_trace_hist with "[$Htr_is]") as "(Htr_is & #Htr_hist)".
+    iMod (lin_tag_create lt t γmlin (#tag1, (c, #"StPre"))%V with "[$Hlin_res]") 
+      as "(Hlin_res & Hlin_tag_res)".
+    {
+      iPureIntro.
+      simpl.
+      do 2 (split; first done).
+      intros Hfalse.
+      destruct Hfalse as [Hfalse | [[Hfalse | Hfalse] | [Hfalse | [Hfalse | Hfalse]]]]; 
+        rewrite /is_st_post_event /is_wr_post_event /is_cm_post_event /is_in_post_event in Hfalse; 
+        set_solver.
+    }
+    iMod (post_tag_create t γmpost (#tag1, (c, #"StPre"))%V with "[$Hpost_res]") 
+      as "(Hpost_res & Hpost_tag_res)".
+    {
+      iPureIntro.
+      simpl.
+      do 2 (split; first done).
+      intros Hfalse.
+      destruct Hfalse as [Hfalse | [[Hfalse | Hfalse] | [Hfalse | [Hfalse | Hfalse]]]]; 
+        rewrite /is_st_post_event /is_wr_post_event /is_cm_post_event /is_in_post_event in Hfalse; 
+        set_solver.
+    }
+    iMod ("Hclose" with "[Htrans_res Htr_is HOwnLin Hstate_res Hlin_res Hpost_res]").
+    {
+      iNext.
+      iExists T.
+      iFrame.
+      iExists (t ++ [(#tag1, (c, #"StPre"))%V]), lt.
+      iFrame.
+      iSplitR; last set_solver.
+      iPureIntro.
+      apply (lin_trace_valid tag1); try done.
+      rewrite /is_pre_event /is_st_pre_event.
+      set_solver.
+    }
+    iModIntro.
+    wp_pures.
+    wp_apply "Hstart"; try done.
+    iClear "Hstart".
+    iMod "Hshift" as "[%m (((Hconn_state & Hsa_pointer) & Hkeys) & Hshift)]".
+    iModIntro.
+    iExists m.
+    iFrame.
+    rewrite big_sepM_sep.
+    iDestruct "Hkeys" as "(Hkeys1 & Hkeys2)".
+    iFrame.
+    iModIntro.
+    iIntros "(Hconn_state & Hkeys1 & Hkeys_conn)".
+    iInv "HinvExt" as ">[%T' (Htrans_res' & [%t' [%lt' 
+      (Htr_is' & HOwnLin' & %HlinOf' & %Hno_empty' & %Hex' & %Hvalid_trans' & 
+      %Hvalid_seq' & HstateRes' & Hlin_res' & Hpost_res')]])]" "Hclose'".
+    simpl; rewrite /trace_state_resources.
+    iDestruct "HstateRes'" as "(%mstate' & Hghost_map_mstate' & %mname' & Hghost_map_mname' & Hdisj_trace_res)".
+    iDestruct (@ghost_map_lookup with "[$Hghost_map_mstate'][$Hsa_pointer]") as "%Hlookup_mstate'".
+    assert (clients = {[sa]} ∪ (clients ∖ {[sa]})) as Heq_sa_clients.
+    {
+      apply union_difference_L.
+      set_solver.
+    }
+    rewrite {3} Heq_sa_clients.
+    rewrite (big_sepS_union _ {[sa]} (clients ∖ {[sa]})); last set_solver.
+    iDestruct "Hdisj_trace_res" as "(Hdisj_trace_res_sa & Hdisj_trace_res)".
+    rewrite big_sepS_singleton.
+    iDestruct "Hdisj_trace_res_sa" as "[(Hfalse & _) | Htrace_res]".
+    {
+      iDestruct "Hfalse" as "[%Hfalse | %Hfalse]"; set_solver.
+    }
+    iDestruct "Htrace_res" as "(%ls & %c' & %γ & %m' & %Hlookup_mstate'' & %Hextract & 
+      #Hsa_c'_pointer & Hghost_map_m' & %Hinit & [(-> & %Hclosed & %Hopen_trans & Hkeys_conn_res) | Hfalse])"; last first.
+    {
+      assert (ls = CanStart) as ->; first set_solver.
+      by iDestruct "Hfalse" as "(%domain & %sub_domain & %tail & %Hfalse & _)".
+    }
+    iMod (ghost_map_update (Active (dom m), Some c) with "[$Hghost_map_mstate'] [$Hsa_pointer]") 
+      as "(Hghost_map_mstate' & Hsa_pointer)".
+    iAssert ((|==> (([∗ set] k ∈ KVS_keys, ghost_map_elem γ k (DfracOwn 1%Qp) None) ∗ 
+              (∃ m'', ghost_map_auth γ 1 m'' ∧ ⌜∀ k, k ∈ KVS_keys → m'' !! k = Some None⌝)))%I) 
+      with "[Hkeys_conn_res Hghost_map_m']" as ">(Hkeys_conn_res & (%m'' & Hghost_map_m' & %Hnone))".
+    {
+      iRevert "Hghost_map_m'".
+      iRevert (m').
+      iInduction KVS_keys as [|k KVS_Keys Hnin] "IH" using set_ind_L.
+      - iIntros (m') "Hghost_map_m'".
+        iModIntro. 
+        iSplitR "Hghost_map_m'"; first done.
+        iExists m'.
+        iFrame.
+        iPureIntro.
+        set_solver.
+      - iIntros (m') "Hghost_map_m'".
+        rewrite big_sepS_union; last set_solver.
+        iDestruct "Hkeys_conn_res" as "(Hkeys_conn_key & Hkeys_conn_res)".
+        iMod ("IH" with "[$Hkeys_conn_res][$Hghost_map_m']") 
+          as "(Hkeys_conn_res & [%m'' (Hghost_map' & %Hnone)])".
+        rewrite big_sepS_singleton.
+        iDestruct "Hkeys_conn_key" as "(%ov & Hkeys_conn_key)".
+        iMod (ghost_map_update None with "[$Hghost_map'] [$Hkeys_conn_key]") 
+          as "(Hghost_map' & Hkeys_conn_key)".
+        iModIntro.
+        iSplitR "Hghost_map'".
+        + rewrite big_sepS_union; last set_solver.
+          iFrame. 
+          rewrite big_sepS_singleton.
+          iFrame.
+        + iExists _.
+          iFrame.
+          iPureIntro.
+          intros k' Hin.
+          destruct (decide (k = k')) as [->|Hneq].
+          * by rewrite lookup_insert.
+          * rewrite lookup_insert_ne; last done.
+            apply Hnone.
+            set_solver.
+    }
+    iAssert ((([∗ set] k ∈ (dom m) ∩ KVS_keys, ghost_map_elem γ k (DfracOwn 1%Qp) None) ∗ 
+              ([∗ set] k ∈ KVS_keys ∖ ((dom m) ∩ KVS_keys), ghost_map_elem γ k (DfracOwn 1%Qp) None))%I) 
+      with "[Hkeys_conn_res]" as "(Hkeys_conn_res1 & Hkeys_conn_res2)".
+    {
+      assert (KVS_keys = (dom m ∩ KVS_keys) ∪ (KVS_keys ∖ (dom m ∩ KVS_keys))) as Heq.
+      - apply union_difference_L.
+        set_solver.
+      - rewrite {1} Heq.
+        rewrite (big_sepS_union _ (dom m ∩ KVS_keys) (KVS_keys ∖ (dom m ∩ KVS_keys))); last set_solver.
+        iFrame.
+    }
+    iMod (own_lin_add _ _ (#tag1, (c, #"StLin"))%V with "[$HOwnLin']") as "HOwnLin'".
+    iMod (own_lin_hist with "[$HOwnLin']") as "(HOwnLin' & #HOwnLinHist')".
+    iPoseProof (trace_hist_trace_is_prefix with "[$Htr_is'][$Htr_hist]") as "%Hprefix".
+    assert ((#tag1, (c, #"StPre"))%V ∈ t') as Hin.
+    {
+      apply (elem_of_prefix (t ++ [(#tag1, (c, #"StPre"))%V])); last done.
+      set_solver.
+    }
+    iPoseProof (lin_tag_not_in lt' t' γmlin with "[$Hlin_res' $Hlin_tag_res]") as "%Hnot_lin_in".
+    iPoseProof (post_tag_not_in t' γmpost with "[$Hpost_res' $Hpost_tag_res]") as "%Hnot_post_in".
+    iDestruct (lin_tag_add lt' t' γmlin (#tag1, (c, #"StLin"))%V tag1 with "[$Hlin_res' $Hlin_tag_res]") 
+      as "Hlin_res'".
+    {
+      iPureIntro.
+      by simpl. 
+    }
+    iMod ("Hclose'" with "[Htrans_res' Htr_is' HOwnLin' Hghost_map_mname' Hghost_map_m' 
+      Hghost_map_mstate' Hkeys_conn_res2 Hlin_res' Hpost_res' Hdisj_trace_res]").
+    {
+      iModIntro.
+      iExists T'.
+      iFrame.
+      iExists t', (lt' ++ [(#tag1, (c, #"StLin"))%V]).
+      iFrame.
+      iSplitR.
+      {
+        iPureIntro.
+        apply (lin_trace_lin lt' ((#tag1, (c, #"StPre"))%V) ((#tag1, (c, #"StLin"))%V) tag1 c t'); 
+          try done; rewrite /is_lin_event /is_pre_event; left; by exists tag1, c.
+      }
+      iSplitR; first by iPureIntro.
+      iSplitR.
+      {
+        iPureIntro.
+        destruct Hex' as (Hex1 & Hex2 & Hex3).
+        split.
+        - intros le op Hle_in Hlin_le.
+          specialize (Hex1 le op).
+          apply Hex1; last done.
+          rewrite elem_of_app in Hle_in.
+          destruct Hle_in as [Hle_in | Hle_in]; first done.
+          assert (le = (#tag1, (c, #"StLin"))%V) as ->; first set_solver.
+          inversion Hlin_le.
+        - split.
+          + intros trans op Hin_t Hin_op.
+            specialize (Hex2 trans op Hin_t Hin_op).
+            set_solver.
+          + intros trans op1 op2 Htrans_in Hrel.
+            specialize (Hex3 trans op1 op2 Htrans_in Hrel).
+            destruct Hex3 as (i & j & Hle & Hlookup_i & Hlookup_j).
+            exists i, j.
+            split; first done.
+            split; by apply lookup_app_l_Some.
+      }
+      iSplitR; first by iPureIntro.
+      iSplitR.
+      {
+        iPureIntro.
+        apply valid_sequence_st_lin; set_solver.
+      }
+      iExists (<[sa:=(Active (dom m), Some c)]> mstate').
+      iFrame.
+      iExists mname'.
+      iFrame.
+      rewrite {3} Heq_sa_clients.
+      rewrite big_sepS_union; last set_solver.
+      iSplitL "Hkeys_conn_res2 Hghost_map_m'".
+      - rewrite big_sepS_singleton.
+        iRight.
+        rewrite /initialized_trace_resources.
+        rewrite lookup_insert.
+        iExists (Active (dom m)), c, γ, m''.
+        assert (c = c') as ->; first set_solver.
+        iFrame "#∗".
+        do 3 (iSplit; first iPureIntro; first set_solver).
+        iRight.
+        iExists (dom m), ((dom m) ∩ KVS_keys), [].
+        do 2 (iSplit; first by iPureIntro).
+        iSplitR.
+        + iPureIntro.
+          exists (#tag1, (c', #"StLin"))%V, lt'.
+          do 2 (split; first done).
+          split; first by exists tag1.
+          set_solver.
+        + iSplitL.
+          * iApply (big_sepS_wand with "[$Hkeys_conn_res2]").
+            iApply big_sepS_intro.
+            iModIntro.
+            iIntros (k Hk_in) "Hkey".
+            iExists None.
+            iFrame.
+          * iIntros (k' Hk'_dom ov Hlookup).
+            iPureIntro.
+            destruct ov as [v|].
+            -- rewrite Hnone in Hlookup; first done.
+               set_solver.
+            -- left.
+               set_solver.
+      - iApply (big_sepS_wand with "[$Hdisj_trace_res]").
+        iApply big_sepS_intro.
+        iModIntro.
+        iIntros (sa' Hsa'_in) "Hsa'".
+        iApply (client_trace_state_resources_neq2 sa sa' c with "[][][][$]"); try done.
+        iPureIntro; set_solver.
+    }
+    iMod ("Hshift" with "[Hkeys1 Hkeys2 Hkeys_conn Hsa_pointer Hkeys_conn_res1 Hconn_state]").
+    {
+      iFrame.
+      do 2 rewrite big_sepM_dom.
+      iInduction (dom m) as [|k dom Hnin] "IH" using set_ind_L; first set_solver.
+      rewrite big_sepS_union; last set_solver.
+      iDestruct "Hkeys_conn" as "(Hkeys_conn_key & Hkeys_conn)".
+      assert (c = c') as <-; first set_solver.
+      destruct (decide (k ∈ KVS_keys)) as [Hk_in | Hk_nin].
+      - assert (({[k]} ∪ dom) ∩ KVS_keys = {[k]} ∪ (dom ∩ KVS_keys)) as ->; first set_solver.
+        rewrite big_sepS_union; last set_solver.
+        iDestruct "Hkeys_conn_res1" as "(Hkeys_conn_res1_key & Hkeys_conn_res1)".
+        iDestruct ("IH" with "[$Hkeys_conn][$Hkeys_conn_res1]") as "Hkeys_conn".
+        rewrite big_sepS_union; last set_solver.
+        iFrame.
+        iDestruct (big_sepS_sep with "[$Hkeys_conn_key $Hkeys_conn_res1_key]") 
+          as "Hkeys_conn_key".
+        iApply (big_sepS_wand with "[$Hkeys_conn_key]").
+        iApply big_sepS_intro.
+        iModIntro.
+        iIntros (key Hin') "Hres".
+        iDestruct "Hres" as "(Hres1 & Hres2)".
+        iFrame.
+        iExists sa, γ.
+        iFrame "#".
+        iSplit; first done.
+        iSplit; last done.
+        iIntros (Hkey_in).
+        iFrame.
+      - assert (({[k]} ∪ dom) ∩ KVS_keys = dom ∩ KVS_keys) as ->; first set_solver.
+        rewrite big_sepS_union; last set_solver.
+        iDestruct ("IH" with "[$Hkeys_conn][$Hkeys_conn_res1]") as "Hkeys_conn".
+        iFrame.
+        iApply (big_sepS_wand with "[$Hkeys_conn_key]").
+        iApply big_sepS_intro.
+        iModIntro.
+        iIntros (key Hin') "Hres".
+        iFrame.
+        iExists sa, γ.
+        iFrame "#".
+        iSplit; first done.
+        iSplitL; last done.
+        iIntros (Hkey_in).
+        set_solver.
+    }
+    iModIntro.
+    rewrite /start_post_emit_event.
+    wp_pures.
+    iInv "HinvExt" as ">[%T'' (Htrans_res'' & [%t'' [%lt'' 
+      (Htr_is'' & HOwnLin'' & %HlinOf'' & %Hno_empty'' & %Hex'' & %Hvalid_trans'' & 
+      %Hvalid_seq'' & HstateRes'' & Hlin_res'' & Hpost_res'')]])]" "Hclose''".
+    iDestruct (own_lin_prefix with "[$HOwnLin'' $HOwnLinHist']") 
+      as "(HOwnLin'' & HOwnLinHist & %Hprefix')".
+    assert ((#tag1, (c, #"StLin"))%V ∈ lt'') as HstLinIn.
+    {
+      apply (elem_of_prefix (lt' ++ [(#tag1, (c, #"StLin"))%V])); last done.
+      set_solver.
+    }
+    wp_apply (aneris_wp_emit with "[$Htr_inv $Htr_is'']").
+    {
+      rewrite Hkvs_inv_name.
+      solve_ndisj.
+    }
+    {
+      (* eapply valid_trace_ru_post; 
+        rewrite /is_post_event /is_st_post_event;
+        set_solver. *)
+      admit.
+    }
+    iIntros "Htr_is''".
+    iDestruct (lin_tag_add_post lt'' t'' γmlin (#tag1, (c, #"StPost"))%V with "[$Hlin_res'']") as "Hlin_res''".
+    iDestruct (post_tag_add t'' γmpost (#tag1, (c, #"StPost"))%V tag1 with "[$Hpost_res'' $Hpost_tag_res]")
+     as "Hpost_res''".
+    {
+      simpl.
+      iSplitL; first by iPureIntro.
+      iPureIntro.
+      left.
+      by eexists _, _.
+    }
+    iMod ("Hclose''" with "[Htrans_res'' Htr_is'' HOwnLin'' HstateRes'' Hlin_res'' Hpost_res'']").
+    {
+      iModIntro.
+      iExists T''.
+      iFrame.
+      iExists (t'' ++ [(#tag1, (c, #"StPost"))%V]), lt''.
+      iFrame.
+      iSplitR; last set_solver.
+      iPureIntro.
+      apply (lin_trace_valid tag1); try done.
+      rewrite /is_post_event /is_st_post_event.
+      set_solver.
+    }
+    set_solver.
+  Admitted.
+
+  Lemma commit_implication γtrans γmstate γmlin γmpost γmname γl clients (res : RC_resources Mdl Σ) 
+  (lib : KVS_transaction_api) : 
+    ⌜KVS_InvName = nroot .@ "kvs_inv"⌝ -∗
+    trace_inv trace_inv_name valid_trace_rc -∗
+    inv KVS_InvName (∃ T, GlobalInvExtRC γtrans T ∗ GlobalInvExt T extract γmstate γmlin γmpost γmname γl clients) -∗
+    @commit_spec _ _ _ _ lib res -∗
+    @commit_spec _ _ _ _ (KVS_wrapped_api lib) (wrapped_resources γtrans γmstate γmlin γmpost γmname γl clients res).
+  Proof.
+  Admitted.
 
   (* Primary lemma to be used with adequacy *)
-  Lemma library_implication `{!anerisG Mdl Σ} (clients : gset socket_address) 
-  (lib : KVS_transaction_api) :
+  Lemma library_implication (clients : gset socket_address) (lib : KVS_transaction_api) :
     ((RC_spec clients lib) ∗ trace_is [] ∗ 
       trace_inv trace_inv_name valid_trace_rc ∗ ⌜KVS_InvName = nroot .@ "kvs_inv"⌝) ={⊤}=∗ 
     RC_spec clients (KVS_wrapped_api lib).
   Proof.
-  Admitted.
+    iIntros "([%res (Hkeys & Hkvs_init & #Hglob_inv & Hcan_conn & 
+      (#Hinit_kvs & #Hinit_cli & #Hread & #Hwrite & #Hstart & #Hcom))] & Htr & #Htr_inv & %Hkvs_inv_name)".    
+    iMod (ghost_map_alloc ((gset_to_gmap (CanStart, None) clients : 
+      gmap socket_address (local_state * option val))))
+      as "[%γmstate (Hghost_map_mstate & Hghost_elems_mstate)]".
+    iMod (ghost_map_alloc_empty (K:=string) (V:=bool)) as "[%γmlin Hghost_map_mlin]".
+    iMod (ghost_map_alloc_empty (K:=string) (V:=bool)) as "[%γmpost Hghost_map_mpost]".
+    iMod (ghost_map_alloc_empty (K:=socket_address) (V:=(gname * val))) as "[%γmname Hghost_map_mname]".
+    iMod (own_alloc (● gmap_of_trace 0 ([] : list val) ⋅ 
+      ◯ gmap_of_trace 0 ([] : list val))) as (γl) "Hltrace".
+    {
+      apply auth_both_valid. 
+      split; first done. 
+      by apply gmap_of_trace_valid.
+    }
+    iDestruct "Hltrace" as "[Hltrace Hlhist]".
+    iMod (own_alloc (● gmap_of_trace 0 ([] : list transaction) ⋅ 
+      ◯ gmap_of_trace 0 ([] : list transaction))) as (γtrans) "Htrans".
+    {
+      apply auth_both_valid. 
+      split; first done. 
+      by apply gmap_of_trace_valid.
+    }
+    iDestruct "Htrans" as "[Htrans Htrans_sub]".
+    iMod (inv_alloc KVS_InvName ⊤ (∃ T, GlobalInvExtRC γtrans T ∗ GlobalInvExt T extract γmstate γmlin γmpost γmname γl clients) with 
+      "[Htr Hghost_map_mstate Hghost_map_mlin Hghost_map_mpost Hghost_map_mname Hltrace Hlhist Htrans Htrans_sub]") as "#HinvExt".
+    {
+      iNext.
+      iExists [].
+      iSplitL "Htrans Htrans_sub".
+      {
+        iSplit; last iPureIntro; last set_solver.
+        rewrite /OwnTrans.
+        iFrame.
+      }
+      iExists [], [].
+      iFrame.
+      simpl.
+      iSplitR.
+      {
+        iPureIntro.
+        rewrite /lin_trace_of /rel_list.
+        set_solver.
+      }
+      iSplitR; first iPureIntro; first set_solver.
+      iSplitR.
+      {
+        iPureIntro.
+        rewrite /extraction_of.
+        set_solver.
+      }
+      iSplitR.
+      {
+        iPureIntro.
+        rewrite /valid_transactions.
+        set_solver.
+      }
+      iSplitR.
+      {
+        iPureIntro.
+        rewrite /valid_sequence /unique_init_events.
+        set_solver.
+      }
+      iClear "Hinit_kvs Hinit_cli Hread Hstart Hwrite Hcom".
+      iSplitR "Hghost_map_mlin Hghost_map_mpost".
+      - iExists (gset_to_gmap (CanStart, None) clients).
+        iFrame.
+        iExists ∅.
+        iFrame.
+        iApply big_sepS_intro.
+        iModIntro.
+        iIntros (sa Hin).
+        iLeft.
+        iSplit.
+        + iRight.
+          iPureIntro.
+          by rewrite lookup_gset_to_gmap_Some.
+        + iSplit.
+          * iPureIntro.
+            set_solver.
+          * iPureIntro.
+            rewrite /no_emit_with_address.
+            set_solver.
+      - iSplitL "Hghost_map_mlin". 
+        + iExists ∅.
+          iFrame.
+          iSplitL; first set_solver.
+          iIntros (tag Hexists). 
+          set_solver.
+        + iExists ∅.
+          iFrame.
+          iSplitL; first set_solver.
+          iIntros (tag Hexists).
+          set_solver.
+    }
+    iModIntro.
+    iExists (wrapped_resources γtrans γmstate γmlin γmpost γmname γl clients res).
+    iFrame "Hkvs_init".
+    iSplitL "Hkeys".
+    {
+      simpl.
+      iApply (big_sepS_mono with "[$Hkeys]").
+      iIntros (k Hin) "Hkey". 
+      iFrame.
+      iSplit; by iIntros (v) "%Hfalse".
+    }
+    iSplitR; iFrame "∗#".
+    iSplitL "Hghost_elems_mstate Hcan_conn".
+    {
+      simpl.
+      rewrite big_sepM_gset_to_gmap.
+      rewrite big_sepS_sep.
+      iFrame.
+      iApply (big_sepS_mono with "[$Hghost_elems_mstate]").
+      iIntros (sa Hin) "Hkey".
+      by iFrame.
+    }
+    iSplitR.
+    {
+      iClear "Hinit_kvs Hstart Hwrite Hread Hcom".
+      iApply (init_client_implication with "[//][$Htr_inv][$HinvExt][$Hinit_cli]").
+    }
+    iSplitR.
+    {
+      iClear "Hinit_kvs Hinit_cli Hwrite Hstart Hcom".
+      iApply (read_implication with "[//][$Htr_inv][$HinvExt][]").
+      iIntros (c sa E k) "!# #Hsub #Hin #Hconn %Φ !# Hshift".
+      iApply ("Hread" $! c sa E k with "[$][$][$][$Hshift]").
+    }
+    iSplitR.
+    {
+      iClear "Hinit_kvs Hinit_cli Hread Hstart Hcom".
+      iApply (write_implication with "[//][$Htr_inv][$HinvExt][]").
+      iIntros (c sa E k v) "!# #Hsub #Hin #Hconn %Φ !# Hshift".
+      iApply ("Hwrite" $! c sa E k v with "[$][$][$][$Hshift]").
+    }
+    iSplitR.
+    {
+      iClear "Hinit_kvs Hinit_cli Hwrite Hread Hcom".
+      iApply (start_implication with "[//][$Htr_inv][$HinvExt][]").
+      iIntros (c sa E) "!# #Hsub #Hconn %Φ !# Hshift".
+      iApply ("Hstart" $! c sa E with "[$][$][$Hshift]").
+    }
+    iClear "Hinit_kvs Hinit_cli Hwrite Hread Hstart".
+    iApply (commit_implication with "[//][$Htr_inv][$HinvExt][]").
+    iIntros (c sa E) "!# #Hsub #Hconn %Φ !# Hshift".
+    iApply ("Hcom" $! c sa E with "[$][$][$Hshift]").
+  Qed.
 
 End trace_proof.
